commit

AP/System/Symmetry.lean
@@ -1,5 +1,26 @@
 import AP.System.Invariant
 
+namespace Equiv
+
+variable {α β γ : Type*}
+variable {e : α ≃ β} {e₁ : β ≃ γ} {e₂ : α ≃ β}
+
+def comp (e₁ : β ≃ γ) (e₂ : α ≃ β) : α ≃ γ where
+  toFun := e₁ ∘ e₂
+  invFun := e₂.symm ∘ e₁.symm
+  left_inv := by intros x; simp
+  right_inv := by intros x; simp
+
+@[simp]
+theorem coe_toFun_comp : (e₁.comp e₂ : _ → _) = e₁ ∘ e₂ := rfl
+
+@[simp]
+theorem symm_comp : (e₁.comp e₂).symm = e₂.symm.comp e₁.symm := rfl
+
+-- #check 0 #exit
+
+end Equiv
+
 namespace System
 
 universe u
@@ -14,21 +35,29 @@ structure Symmetry (sys : System S T) : Type u where
 
 namespace Symmetry
 
-variable {sym : sys.Symmetry}
+variable {sym sym₁ sym₂ : sys.Symmetry}
 
 class WF (sym : sys.Symmetry) : Prop where
-  h_fs : Function.BijectiveOn sys.WF sys.WF sym.fs sym.fs'
-  h_ft : Function.BijectiveOn sys.WFTrans sys.WFTrans sym.ft sym.ft'
+  h_fs : BijectiveOn sys.WF sys.WF sym.fs sym.fs'
+  h_ft : BijectiveOn sys.WFTrans sys.WFTrans sym.ft sym.ft'
   tr_eq : ∀ {s t} [sys.WF s], sys.tr s t = (sys.tr (sym.fs s) (sym.ft t)).map sym.fs'
   tr_eq' : ∀ {s t} [sys.WF s], sys.tr s t = (sys.tr (sym.fs' s) (sym.ft' t)).map sym.fs
 
-instance : Inhabited (Symmetry sys) := ⟨id, id, id, id⟩
+def zero : sys.Symmetry := ⟨id, id, id, id⟩
 
-theorem default_eq : (default : Symmetry sys) = ⟨id, id, id, id⟩ := rfl
+instance : Zero sys.Symmetry := ⟨zero⟩
+theorem zero_def : (0 : sys.Symmetry) = zero := rfl
+
+instance : Inhabited sys.Symmetry := ⟨zero⟩
+theorem default_eq : (default : sys.Symmetry) = 0 := rfl
 
 @[simp]
-instance : (default : Symmetry sys).WF := by
-  rw [default_eq]; constructor <;> simp
+instance : (0 : sys.Symmetry).WF := by
+  rw [zero_def, zero]; constructor <;> simp
+
+@[simp]
+instance : (default : sys.Symmetry).WF := by
+  rw [default_eq]; infer_instance
 
 instance {s} [H : sym.WF] [hs : sys.WF s] : sys.WF (sym.fs s) :=
   H.h_fs.cnd_right hs
@@ -131,29 +160,96 @@ sys.validTr (sym.fs s) t ↔ sys.validTr s (sym.ft' t) := by
   · exact fun a ↦ validTr_ft'_of a
 
 @[simp]
-def simFn (sym : Symmetry sys) (f : S → T) (s : S) : T :=
+def simFn (sym : sys.Symmetry) (f : S → T) (s : S) : T :=
   sym.ft # f # sym.fs' s
 
 instance {f} [H : sym.WF] [hf : sys.SimFn f] : sys.SimFn (sym.simFn f) := by
   rw [sys.simFn_def]; intro s hs h; simp; apply hf.1 at h; apply validTr_ft_of
   have h₁ : sys.hasTr (sym.fs' s); simp; exact ⟨_, h⟩; exact hf.1 h₁
 
-def inv (sym : Symmetry sys) : Symmetry sys where
+def neg (sym : sys.Symmetry) : sys.Symmetry where
   fs := sym.fs'
   fs' := sym.fs
   ft' := sym.ft
   ft := sym.ft'
 
-@[simp]
-theorem inv_inv : sym.inv.inv = sym := by ext <;> rfl
+instance : Neg sys.Symmetry := ⟨.neg⟩
+theorem neg_def : -sym = sym.neg := rfl
 
-instance [H : sym.WF] : sym.inv.WF where
+@[simp]
+theorem neg_neg : -(-sym) = sym := by ext <;> rfl
+
+instance [H : sym.WF] : (-sym).WF where
   h_fs := H.h_fs.symm
   h_ft := H.h_ft.symm
   tr_eq := WF.tr_eq'
   tr_eq' := WF.tr_eq
 
 @[simp]
-theorem wf_inv_iff : sym.inv.WF ↔ sym.WF := by
+theorem wf_neg_iff : (-sym).WF ↔ sym.WF := by
   symm; constructor <;> intro h; infer_instance
-  rw [←sym.inv_inv]; infer_instance
+  rw [←sym.neg_neg]; infer_instance
+
+def add (sym₁ sym₂ : sys.Symmetry) : sys.Symmetry where
+  fs := sym₁.fs ∘ sym₂.fs
+  fs' := sym₂.fs' ∘ sym₁.fs'
+  ft := sym₁.ft ∘ sym₂.ft
+  ft' := sym₂.ft' ∘ sym₁.ft'
+
+instance : Add sys.Symmetry := ⟨add⟩
+theorem add_def : sym₁ + sym₂ = sym₁.add sym₂ := rfl
+
+@[simp]
+instance [H₁ : sym₁.WF] [H₂ : sym₂.WF] : (sym₁ + sym₂).WF := by
+  rw [add_def, add]; constructor <;> dsimp
+  · constructor; have ⟨e₁, h₁, h₂⟩ := H₁.h_fs; have ⟨e₂, h₃, h₄⟩ := H₂.h_fs
+    use e₁.comp e₂; constructor <;> intro s hs <;> simp
+    rw [h₃ hs]; apply h₁; rw [h₂ hs]; apply h₄
+  · constructor; have ⟨e₁, h₁, h₂⟩ := H₁.h_ft; have ⟨e₂, h₃, h₄⟩ := H₂.h_ft
+    use e₁.comp e₂; constructor <;> intro s hs <;> simp
+    rw [h₃ hs]; apply h₁; rw [h₂ hs]; apply h₄
+  · intro s t hs; ext s'; simp; constructor
+    · intro h₁; have hs' := wf_of_tr h₁; use sym₁.fs # sym₂.fs s'
+      have ht := wfTrans_of_tr h₁; simp [tr_fs]; use s'
+    · rintro ⟨s', h₁, rfl⟩; have hs₁ := wf_of_tr h₁; simp [tr_ft] at h₁
+      obtain ⟨s', h₁, rfl⟩ := h₁; have hs' := wf_of_tr h₁; simpa
+  · intro s t hs; ext s'; simp; constructor
+    · intro h₁; have hs' := wf_of_tr h₁; use sym₂.fs' # sym₁.fs' s'
+      have ht := wfTrans_of_tr h₁; simp [tr_fs']; use s'
+    · rintro ⟨s', h₁, rfl⟩; have hs₁ := wf_of_tr h₁; simp [tr_ft'] at h₁
+      obtain ⟨s', h₁, rfl⟩ := h₁; have hs' := wf_of_tr h₁; simpa
+
+def mulNat (sym : sys.Symmetry) (n : ℕ) : sys.Symmetry :=
+  (sym + ·)^[n] 0
+
+def mulInt (sym : sys.Symmetry) : ℤ → sys.Symmetry
+| .ofNat n => sym.mulNat n
+| .negSucc n => (-sym).mulNat # n + 1
+
+theorem zero_add : 0 + sym = sym := rfl
+theorem add_zero : sym + 0 = sym := rfl
+theorem add_assoc {s₁ s₂ s₃ : sys.Symmetry} : s₁ + s₂ + s₃ = s₁ + (s₂ + s₃) := rfl
+
+instance : AddMonoid sys.Symmetry where
+  zero_add := λ _ => zero_add
+  add_zero := λ _ => add_zero
+  add_assoc := λ _ _ _ => add_assoc
+  nsmul := λ n sym => sym.mulNat n
+  nsmul_succ := by
+    intro n sym; simp_rw [mulNat, Function.iterate_succ']; simp
+    induction n; rfl; nm n ih; rw [Function.iterate_succ']; simp [←add_assoc, ih]
+
+#check 0 #exit
+
+theorem nsmul_neg {n} : -sym n = -sym.mulNat n := by
+  sorry
+
+-- #check 0 #exit
+
+instance : SubNegMonoid sys.Symmetry where
+  zsmul := λ n sym => sym.mulInt n
+  zsmul_succ' := AddMonoid.nsmul_succ
+  zsmul_neg' := by
+    clear sym sym₁ sym₂
+    intro n sym
+    simp [mulInt]
